Safety from base

HappensBefore.v
@@ -9,7 +9,7 @@ From Elo Require Import GCR.
 From Elo Require Import SafetyLemmas.
 From Elo Require Import SafetyUtil.
 
-Notation "'<<' ev1 ',' tc ',' ev2 '>>'" := (ev2 :: tc +++ ev1).
+Notation "'<(' ev1 '-{' tc '}-' ev2 ')>'" := (ev2 :: tc +++ ev1).
 
 (* ------------------------------------------------------------------------- *)
 (* happens-before                                                            *)
@@ -17,42 +17,36 @@ Notation "'<<' ev1 ',' tc ',' ev2 '>>'" := (ev2 :: tc +++ ev1).
 
 Inductive happens_before : trace -> Prop :=
   | hb_thread : forall tc tid e1 e2,
-    happens_before ((tid, e2) :: tc +++ (tid, e1))
+    happens_before <((tid, e1) -{tc}- (tid, e2))>
 
   | hb_release_acquire : forall tc tid1 tid2 ad e1 e2,
     is_release ad e1 ->
     is_acquire ad e2 ->
-    happens_before ((tid2, e2) :: tc +++ (tid1, e1))
+    happens_before <((tid1, e1) -{tc}- (tid2, e2))>
 
   | hb_initialize_acquire : forall tc tid1 tid2 ad t e,
     is_acquire ad e ->
-    happens_before ((tid2, e) :: tc +++ (tid1, e_init ad t))
+    happens_before <((tid1, e_init ad t) -{tc}- (tid2, e))>
 
   | hb_transitivity : forall tcA tcB ev1 ev2 ev3,
-    happens_before (ev2 :: tcA +++ ev1) ->
-    happens_before (ev3 :: tcB +++ ev2) ->
-    happens_before (ev3 :: tcB ++ ev2 :: tcA +++ ev1)
+    happens_before <(ev1 -{tcA              }- ev2)> ->
+    happens_before <(ev2 -{tcB              }- ev3)> ->
+    happens_before <(ev1 -{tcB ++ ev2 :: tcA}- ev3)>
   .
 
 (* lemmas ------------------------------------------------------------------ *)
 
 Local Lemma happens_before_from_initialize_then_acquire :
-  forall tc tc1 tc2 tc3 tid1 tid2 e1 e2 eAcq eInit ad t,
+  forall tc tc1 tc2 tc3 tid1 tid2 e1 e2 eAcq ad t,
     is_acquire ad eAcq  ->
-    eInit = e_init ad t ->
-    tc = (tc3 ++ (tid2, eAcq) :: tc2 ++ (tid1, eInit) :: tc1) ->
-    happens_before <<(tid1, e1), tc, (tid2, e2)>>.
+    tc = (tc3 ++ (tid2, eAcq) :: tc2 ++ (tid1, e_init ad t) :: tc1) ->
+    happens_before <((tid1, e1) -{tc}- (tid2, e2))>.
 Proof.
-  intros * ? ? Htc.
+  intros * ? Htc.
   rewrite app_comm_cons in Htc. rewrite app_assoc in Htc.
   remember (tc3 ++ (tid2, eAcq) :: tc2) as tc' eqn: Htc'.
-  rewrite Htc. clear Htc.
-  unfold add. rewrite <- app_assoc. rewrite <- app_comm_cons.
-  eapply hb_transitivity; eauto using happens_before.
-  rewrite Htc'. clear Htc'.
-  unfold add. rewrite <- app_assoc. rewrite <- app_comm_cons.
-  subst.
-  eapply hb_transitivity; eauto using happens_before.
+  rewrite Htc.  eapply hb_transitivity; eauto using happens_before.
+  rewrite Htc'. eapply hb_transitivity; eauto using happens_before.
 Qed.
 
 Local Lemma happens_before_from_release_then_acquire :
@@ -60,18 +54,13 @@ Local Lemma happens_before_from_release_then_acquire :
     is_acquire ad eAcq ->
     is_release ad eRel ->
     tc = (tc3 ++ (tid2, eAcq) :: tc2 ++ (tid1, eRel) :: tc1) ->
-    happens_before <<(tid1, e1), tc, (tid2, e2)>>.
+    happens_before <((tid1, e1) -{tc}- (tid2, e2))>.
 Proof.
   intros * ? ? Htc.
   rewrite app_comm_cons in Htc. rewrite app_assoc in Htc.
   remember (tc3 ++ (tid2, eAcq) :: tc2) as tc' eqn: Htc'.
-  rewrite Htc. clear Htc.
-  unfold add. rewrite <- app_assoc. rewrite <- app_comm_cons.
-  eapply hb_transitivity; eauto using happens_before.
-  rewrite Htc'. clear Htc'.
-  unfold add. rewrite <- app_assoc. rewrite <- app_comm_cons.
-  subst.
-  eapply hb_transitivity; eauto using happens_before.
+  rewrite Htc.  eapply hb_transitivity; eauto using happens_before.
+  rewrite Htc'. eapply hb_transitivity; eauto using happens_before.
 Qed.
 
 (* ------------------------------------------------------------------------- *)
@@ -214,7 +203,7 @@ Local Lemma oneinit_multistep_onecr :
     one_init ad ths1[tid1]         ->
     m1 \ ths1 ~~[tc]~~>* m2 \ ths2 ->
     holding ad ths2[tid2]          ->
-    happens_before <<(tid1, e1), tc, (tid2, e2)>>.
+    happens_before <((tid1, e1) -{tc}- (tid2, e2))>.
 Proof.
   intros.
   assert (exists e tc2 tc3, is_acquire ad e /\ tc = tc3 ++ (tid2, e) :: tc2)
@@ -370,7 +359,7 @@ Local Lemma onecr_multistep_onecr :
     holding ad ths1[tid1]          ->
     m1 \ ths1 ~~[tc]~~>* m2 \ ths2 ->
     holding ad ths2[tid2]          ->
-    happens_before <<(tid1, e1), tc, (tid2, e2)>>.
+    happens_before <((tid1, e1) -{tc}- (tid2, e2))>.
 Proof.
   intros.
   assert (exists e tc2 tc3, is_acquire ad e /\ tc = tc3 ++ (tid2, e) :: tc2)
@@ -406,7 +395,7 @@ Theorem happens_before_from_gcr : forall m1 m2 ths1 ths2 tid1 tid2 e1 e2 tc ad,
   no_reacq ad ths1[tid1]                ->
   no_reacq ad ths2[tid2]                ->
   m1 \ ths1 ~~[tc]~~>* m2 \ ths2        ->
-  happens_before <<(tid1, e1), tc, (tid2, e2)>>.
+  happens_before <((tid1, e1) -{tc}- (tid2, e2))>.
 Proof.
   intros * ? ? ? Hgcr1 Hgcr2 ? ? Hustep.
   assert (forall_threads ths1 term_init_cr_exc) by eauto with inva.
